Simplify array file.

theories/logrel/array.v
@@ -3,12 +3,13 @@ From iris_ni.logrel Require Import types interp.
 From iris_ni.program_logic Require Import dwp heap_lang_lifting.
 From iris.proofmode Require Import tactics.
 From iris_ni.proofmode Require Import dwp_tactics.
-From iris.heap_lang Require Import lang array proofmode.
+From iris.heap_lang Require Import lang array proofmode lib.arith.
 
 (* make : int^low → array τ *)
 (* XXX: how to handle the side condition that n > 0 ? *)
 Definition make : val := λ: "n" "dummy",
-  (AllocN "n" "dummy", "n").
+  let: "n" := maximum "n" #0 in
+  (AllocN (#1 + "n") "dummy", "n").
 
 (* length : array τ → int^low *)
 Definition length : val := λ: "arr",
@@ -18,22 +19,17 @@ Definition length : val := λ: "arr",
 Definition set : val := λ: "arr" "i" "v",
   let: "a" := Fst "arr" in
   let: "n" := Snd "arr" in
-  let: "p" := "a" +ₗ "i" in
-  (* XXX: the || is lazy, so we have to ANF this.. *)
-  let: "b1" := ("i" < #0) in
-  if: (("n" ≤ "i") || "b1")
-  then Skip
-  else "p" <- "v".
+  let: "ii" := "i" + #1 in
+  let: "iii" := if: BinOp AndOp (#0 ≤ "i") ("i" < "n") then "ii" else #0 in
+  "a" +ₗ "iii" <- "v".
 
 (* get : array τ → int^α → τ → τ *)
 Definition get : val := λ: "arr" "i" "dummy",
   let: "a" := Fst "arr" in
   let: "n" := Snd "arr" in
-  (* XXX: the || is lazy, so we have to ANF this.. *)
-  let: "b1" := ("i" < #0) in
-  if: (("n" ≤ "i") || "b1") then
-    let: "v" := "dummy" in "v"
-  else !("a" +ₗ "i").
+  let: "ii" := "i" + #1 in
+  let: "iii" := if: BinOp AndOp (#0 ≤ "i") ("i" < "n") then "ii" else #0 in
+  !("a" +ₗ "iii").
 
 Section lookup_total.
   Context {A : Type}.
@@ -53,7 +49,6 @@ Section lookup_total.
     intros Hij.
     rewrite !list_lookup_total_alt list_lookup_insert_ne //.
   Qed.
-
 End lookup_total.
 
 Section spec.
@@ -62,6 +57,9 @@ Section spec.
   Implicit Types n : nat.
   Implicit Types i j : Z.
   Implicit Types v w : val.
+
+  Hint Extern 0 (_ !! _ = _) =>
+    apply list_lookup_lookup_total_lt; lia : core.
 
   (** The array specs are valid only for arrays over the semantic
   types satisfying those conditions. All "flat" types satisfy those.
@@ -72,65 +70,53 @@ Section spec.
   Definition contractible A ξ :=
     (∀ v1 v2, A ξ v1 v1 ∗ A ξ v2 v2 -∗ A ξ v1 v2).
 
-
-  (** * Interpretation *)
-  Definition lrel_list (A : lrel Σ) ξ (vs1 vs2 : list val) :=
-    ([∗ list] i ↦ v1;v2 ∈ vs1;vs2, A ξ v1 v2)%I.
-
   (* XXX: use vectors instead of lists? *)
   Definition array_inv A ξ l1 l2 n :=
     inv (locsN.@(l1,l2))
         (∃ vs1 vs2, ⌜List.length vs1 = n⌝ ∗
                     ⌜List.length vs2 = n⌝ ∗
-                     l1 ↦ₗ∗ vs1 ∗ l2 ↦ᵣ∗ vs2 ∗
-                     lrel_list A ξ vs1 vs2)%I.
+                    l1 ↦ₗ∗ vs1 ∗ l2 ↦ᵣ∗ vs2 ∗
+                    [∗ list] i ↦ v1;v2 ∈ vs1;vs2, A ξ v1 v2)%I.
   Definition lrel_array (A : lrel Σ) : lrel Σ := LRel (λ ξ w1 w2,
-    ∃ (l1 l2 : loc) (n : nat), ⌜w1 = (#l1, #n)%V⌝ ∧ ⌜w2 = (#l2, #n)%V⌝ ∧
-     array_inv A ξ l1 l2 n)%I.
+    ∃ (l1 l2 : loc) (n : nat),
+      ⌜w1 = (#l1, #n)%V⌝ ∧ ⌜w2 = (#l2, #n)%V⌝ ∧
+      array_inv A ξ l1 l2 (S n))%I.
 
   (** * Make typing *)
-  Lemma make_spec (n : nat) v1 v2 A ξ :
-    0 < n →
+  Lemma make_spec (n : Z) v1 v2 A ξ :
     A ξ v1 v2 -∗
     DWP make #n v1 & make #n v2 : lrel_array A ξ.
   Proof.
-    iIntros (?) "#Hv". dwp_rec. dwp_pures.
+    iIntros "#Hv".
+    iAssert (∀ n : Z, ⌜ 0 ≤ n ⌝ →
+      DWP (AllocN #(1 + n) v1, #n) & (AllocN #(1 + n) v2, #n) : lrel_array A ξ)%I as "H"; last first.
+    { rewrite /make /maximum. dwp_pures.
+      case_bool_decide; dwp_pures; iApply "H"; auto with lia. }
+    clear n. iIntros (n' Hn).
+    assert (∃ n : nat, n' = n) as [n ->] by (exists (Z.to_nat n'); lia).
+    rewrite -(Nat2Z.inj_add 1) /=.
     dwp_bind (AllocN _ _) (AllocN _ _).
     (* allocN spec *)
-    set (meta_token1 := @meta_token _ _ _ _ _ heapDG_gen_heapG1).
-    set (meta_token2 := @meta_token _ _ _ _ _ heapDG_gen_heapG2).
-    pose (Ψ1 := (λ v, ∃ l : loc, ⌜v = #l⌝ ∗ l ↦ₗ∗ replicate n v1 ∗
-                 ([∗ list] i ∈ seq 0 n, meta_token1 (l +ₗ Z.of_nat i) ⊤))%I).
-    pose (Ψ2 := (λ v, ∃ l : loc, ⌜v = #l⌝ ∗ l ↦ᵣ∗ replicate n v2 ∗
-                 ([∗ list] i ∈ seq 0 n, meta_token2 (l +ₗ Z.of_nat i) ⊤))%I).
+    pose (Ψ1 v := (∃ l : loc, ⌜v = #l⌝ ∗ l ↦ₗ∗ replicate (S n) v1)%I).
+    pose (Ψ2 v := (∃ l : loc, ⌜v = #l⌝ ∗ l ↦ᵣ∗ replicate (S n) v2)%I).
     iApply (dwp_atomic_lift_wp Ψ1 Ψ2).
     { iApply twp_allocN; try done.
-      iIntros (l) "[Hl Hmeta]". iExists l.
-      iSplit; eauto.
-      rewrite !Nat2Z.id. iSplitL "Hl".
-      iExact "Hl". iFrame. }
+      iIntros (l) "[Hl _]". iExists l. rewrite !Nat2Z.id. by iSplit. }
     { iApply twp_allocN; try done.
-      iIntros (l) "[Hl Hmeta]". iExists l.
-      iSplit; eauto.
-      rewrite !Nat2Z.id. iSplitL "Hl".
-      iExact "Hl". iFrame. }
-    iIntros (? ?). iDestruct 1 as (l1) "[-> [Hl1 Hmeta1]]".
-    iDestruct 1 as (l2) "[-> [Hl2 Hmeta2]]".
+      iIntros (l) "[Hl _]". iExists l. rewrite !Nat2Z.id. by iSplit. }
+    iDestruct 1 as (l1 ->) "Hl1"; iDestruct 1 as (l2 ->) "Hl2".
     (* / allocN spec *)
-    iClear "Hmeta1 Hmeta2".
-
     iNext. dwp_pures. iApply dwp_value.
     iMod (inv_alloc (locsN.@(l1,l2)) _ (∃ vs1 vs2,
-                      ⌜List.length vs1 = n⌝ ∗
-                      ⌜List.length vs2 = n⌝ ∗
+                      ⌜List.length vs1 = S n⌝ ∗
+                      ⌜List.length vs2 = S n⌝ ∗
                       l1 ↦ₗ∗ vs1 ∗ l2 ↦ᵣ∗ vs2 ∗
-                      lrel_list A ξ vs1 vs2)%I with "[-]")
+                      [∗ list] i ↦ v1;v2 ∈ vs1;vs2, A ξ v1 v2)%I with "[-]")
       as "#Hinv".
-    { iNext. iExists _,_. iFrame.
-      rewrite !replicate_length; repeat iSplit; try done.
-      rewrite /lrel_list. clear.
-      induction n; simpl; eauto with iFrame. }
-    iModIntro. iExists _,_,_. repeat iSplit; eauto with iFrame.
+    { iNext. iExists (replicate (S n) v1), (replicate (S n) v2). iFrame.
+      rewrite !replicate_length. do 2 (iSplit; [done|]).
+      induction (S n); simpl; eauto with iFrame. }
+    iModIntro. iEval rewrite /lrel_car /=. eauto 20 with iFrame.
   Qed.
 
   (** * Length typing *)
@@ -143,163 +129,6 @@ Section spec.
   Qed.
 
   (** * Get typing *)
-
-  (** ** For the case when the index is a low integer *)
-  Lemma get_spec_low (a1 a2 : val) v1 v2 d1 d2 A ξ :
-    lrel_array A ξ a1 a2 -∗
-    ⟦ tint Low ⟧ ξ v1 v2 -∗
-    A ξ d1 d2 -∗
-    DWP get a1 v1 d1 & get a2 v2 d2 : A ξ.
-  Proof.
-    iDestruct 1 as (l1 l2 n -> ->) "Ha".
-    iDestruct 1 as (i1 i2 -> ->) "%".
-    assert (i1 = i2) as ->.
-    { by destruct ξ; eauto. }
-    iIntros "Hdummy".
-    dwp_rec. dwp_pures.
-    repeat case_bool_decide; dwp_pures;
-     try by iApply dwp_value.
-    iApply dwp_atomic.
-    iInv (locsN.@(l1, l2)) as
-        (vs1 vs2) "(>% & >% & >Hl1 & >Hl2 & HAs)" "Hcl".
-    rewrite /lrel_list.
-    assert (vs1 !! Z.to_nat i2 = Some (vs1 !!! Z.to_nat i2)) as Hvs1.
-    { apply list_lookup_lookup_total_lt.
-      (* TODO: lia doesn't work here *)
-      rewrite H2. rewrite -(Nat2Z.id n).
-      apply Z2Nat.inj_lt; try lia. }
-    assert (vs2 !! Z.to_nat i2 = Some (vs2 !!! Z.to_nat i2)) as Hvs2.
-    { apply list_lookup_lookup_total_lt.
-      (* TODO: lia doesn't work here *)
-      rewrite H3. rewrite -(Nat2Z.id n).
-      apply Z2Nat.inj_lt; try lia. }
-    pose (Ψ1 := (λ v, ⌜v = vs1 !!! Z.to_nat i2⌝ ∗ l1 ↦ₗ∗ vs1)%I).
-    pose (Ψ2 := (λ v, ⌜v = vs2 !!! Z.to_nat i2⌝ ∗ l2 ↦ᵣ∗ vs2)%I).
-    iApply (dwp_atomic_lift_wp Ψ1 Ψ2 with "[Hl1] [Hl2] [-]").
-    { rewrite /TWP1 /Ψ1.
-      (* TODO: why do I have to specify heapG here? *)
-      iPoseProof (twp_load_offset
-                    (heapG0:=heapG1) with "Hl1") as "HH"; first done.
-      rewrite Z2Nat.id; try lia. iApply "HH". eauto with iFrame. }
-    { rewrite /TWP2 /Ψ2.
-      iPoseProof (twp_load_offset
-                    (heapG0:=heapG2) with "Hl2") as "HH"; first done.
-      rewrite Z2Nat.id; try lia. iApply "HH". eauto with iFrame. }
-    iIntros (??). iDestruct 1 as (->) "Hl1". iDestruct 1 as (->) "Hl2".
-    iNext.
-    iAssert (A ξ (vs1 !!! Z.to_nat i2) (vs2 !!! Z.to_nat i2)) as "#HvsA".
-    { iApply (big_sepL2_lookup with "HAs").
-      apply Hvs1. apply Hvs2. }
-    iMod ("Hcl" with "[-]") as "_".
-    { iNext. iExists _,_. iFrame "Hl1 Hl2 HAs".
-      repeat iSplit; eauto with iFrame. }
-    done.
-  Qed.
-
-  Local Instance id_beta_val_atomic (v : val) :
-    Atomic StronglyAtomic ((λ: "v", "v")%V v).
-  Proof.
-    apply strongly_atomic_atomic, ectx_language_atomic;
-    [inversion 1; naive_solver
-    |apply ectxi_language_sub_redexes_are_values; intros [] **; naive_solver].
-  Qed.
-
-  (** ** Helper lemmas *)
-  Lemma array_get_rhs A ξ (d1 d2 : val) l1 l2 i2 n :
-    pseudo_refl A ξ →
-    contractible A ξ →
-    0 ≤ i2 < n →
-    A ξ d1 d2 -∗
-    array_inv A ξ l1 l2 n -∗
-    DWP (λ: "v", "v")%V d1 & !#(l2 +ₗ i2) : A ξ.
-  Proof.
-    iIntros (PR C Hi2) "#Hdummy Ha".
-    iApply dwp_atomic.
-    iInv (locsN.@(l1, l2)) as
-        (vs1 vs2) "(>% & >% & >Hl1 & >Hl2 & HAs)" "Hcl".
-    rewrite /lrel_list.
-    assert (vs1 !! Z.to_nat i2 = Some (vs1 !!! Z.to_nat i2)) as Hvs1.
-    { apply list_lookup_lookup_total_lt.
-      (* TODO: lia doesn't work here *)
-      rewrite H. rewrite -(Nat2Z.id n).
-      apply Z2Nat.inj_lt; try lia. }
-    assert (vs2 !! Z.to_nat i2 = Some (vs2 !!! Z.to_nat i2)) as Hvs2.
-    { apply list_lookup_lookup_total_lt.
-      (* TODO: lia doesn't work here *)
-      rewrite H0. rewrite -(Nat2Z.id n).
-      apply Z2Nat.inj_lt; try lia. }
-    iModIntro.
-    pose (Ψ1 := (λ v, ⌜v = d1⌝ : iProp Σ)%I).
-    pose (Ψ2 := (λ v, ⌜v = vs2 !!! Z.to_nat i2⌝ ∗ l2 ↦ᵣ∗ vs2)%I).
-    iApply (dwp_atomic_lift_wp Ψ1 Ψ2 with "[] [Hl2] [-]").
-    { rewrite /TWP1 /Ψ1. wp_pures. done. }
-    { rewrite /TWP2 /Ψ2.
-      assert (i2 < n) by lia.
-      iPoseProof (twp_load_offset
-                    (heapG0:=heapG2) with "Hl2") as "HH"; first done.
-      rewrite Z2Nat.id; try lia. (*XXX*)
-      iApply "HH"; eauto. }
-    iIntros (v1 v2 ->). iDestruct 1 as (->) "Hl2".
-    iNext.
-    iAssert (A ξ (vs1 !!! Z.to_nat i2) (vs2 !!! Z.to_nat i2)) as "#HvsA".
-    { iApply (big_sepL2_lookup with "HAs").
-      apply Hvs1. apply Hvs2. }
-    iMod ("Hcl" with "[-]") as "_".
-    { iNext. iExists _,_. iFrame "Hl1 Hl2 HAs".
-      repeat iSplit; eauto with iFrame. }
-    iModIntro. iApply C. iSplit.
-    - rewrite (PR d1 d2). iDestruct "Hdummy" as "[$ _]".
-    - rewrite (PR (vs1 !!! _)). iDestruct "HvsA" as "[_ $]".
-  Qed.
-
-  Lemma array_get_lhs A ξ (d1 d2 : val) l1 l2 i1 n :
-    pseudo_refl A ξ →
-    contractible A ξ →
-    0 ≤ i1 < n →
-    A ξ d1 d2 -∗
-    array_inv A ξ l1 l2 n -∗
-    DWP !#(l1 +ₗ i1) & (λ: "v", "v")%V d2 : A ξ.
-  Proof.
-    iIntros (PR C Hi1) "#Hdummy Ha".
-    iApply dwp_atomic.
-    iInv (locsN.@(l1, l2)) as
-        (vs1 vs2) "(>% & >% & >Hl1 & >Hl2 & HAs)" "Hcl".
-    rewrite /lrel_list.
-    assert (vs1 !! Z.to_nat i1 = Some (vs1 !!! Z.to_nat i1)) as Hvs1.
-    { apply list_lookup_lookup_total_lt.
-      (* TODO: lia doesn't work here *)
-      rewrite H. rewrite -(Nat2Z.id n).
-      apply Z2Nat.inj_lt; try lia. }
-    assert (vs2 !! Z.to_nat i1 = Some (vs2 !!! Z.to_nat i1)) as Hvs2.
-    { apply list_lookup_lookup_total_lt.
-      (* TODO: lia doesn't work here *)
-      rewrite H0. rewrite -(Nat2Z.id n).
-      apply Z2Nat.inj_lt; try lia. }
-    iModIntro.
-    pose (Ψ1 := (λ v, ⌜v = vs1 !!! Z.to_nat i1⌝ ∗ l1 ↦ₗ∗ vs1)%I).
-    pose (Ψ2 := (λ v, ⌜v = d2⌝ : iProp Σ)%I).
-    iApply (dwp_atomic_lift_wp Ψ1 Ψ2 with "[Hl1] [] [-]").
-    { rewrite /TWP1 /Ψ1.
-      assert (i1 < n) by lia.
-      iPoseProof (twp_load_offset
-                    (heapG0:=heapG1) with "Hl1") as "HH"; first done.
-      rewrite Z2Nat.id; try lia. (*XXX*)
-      iApply "HH"; eauto. }
-    { rewrite /TWP2 /Ψ2. wp_pures. done. }
-
-    iIntros (v1 v2). iDestruct 1 as (->) "Hl1". iIntros (->).
-    iNext.
-    iAssert (A ξ (vs1 !!! Z.to_nat i1) (vs2 !!! Z.to_nat i1)) as "#HvsA".
-    { iApply (big_sepL2_lookup with "HAs").
-      apply Hvs1. apply Hvs2. }
-    iMod ("Hcl" with "[-]") as "_".
-    { iNext. iExists _,_. iFrame "Hl1 Hl2 HAs".
-      repeat iSplit; eauto with iFrame. }
-    iModIntro. iApply C. iSplit.
-    - rewrite (PR (vs1 !!! _)). iDestruct "HvsA" as "[$ _]".
-    - rewrite (PR d1 d2). iDestruct "Hdummy" as "[_ $]".
-  Qed.
-
   Lemma array_get_both A ξ l1 l2 i1 i2 n :
     pseudo_refl A ξ →
     contractible A ξ →
@@ -309,63 +138,33 @@ Section spec.
     DWP !#(l1 +ₗ i1) & !#(l2 +ₗ i2) : A ξ.
   Proof.
     iIntros (PR C Hi1 Hi2) "Ha".
+    assert (∃ i1' : nat, i1 = i1' ∧ i1' < n)%nat as (i1' & -> & ?)
+      by (exists (Z.to_nat i1); lia).
+    assert (∃ i2' : nat, i2 = i2' ∧ i2' < n)%nat as (i2' & -> & ?)
+      by (exists (Z.to_nat i2); lia).
     iApply dwp_atomic.
     iInv (locsN.@(l1, l2)) as
         (vs1 vs2) "(>% & >% & >Hl1 & >Hl2 & HAs)" "Hcl".
-    rewrite /lrel_list.
-    assert (vs1 !! Z.to_nat i1 = Some (vs1 !!! Z.to_nat i1)) as Hvs1.
-    { apply list_lookup_lookup_total_lt.
-      (* TODO: lia doesn't work here *)
-      rewrite H. rewrite -(Nat2Z.id n).
-      apply Z2Nat.inj_lt; try lia. }
-    assert (vs2 !! Z.to_nat i1 = Some (vs2 !!! Z.to_nat i1)) as Hvs2.
-    { apply list_lookup_lookup_total_lt.
-      (* TODO: lia doesn't work here *)
-      rewrite H0. rewrite -(Nat2Z.id n).
-      apply Z2Nat.inj_lt; try lia. }
-    assert (vs1 !! Z.to_nat i2 = Some (vs1 !!! Z.to_nat i2)) as Hvs1'.
-    { apply list_lookup_lookup_total_lt.
-      (* TODO: lia doesn't work here *)
-      rewrite H. rewrite -(Nat2Z.id n).
-      apply Z2Nat.inj_lt; try lia. }
-    assert (vs2 !! Z.to_nat i2 = Some (vs2 !!! Z.to_nat i2)) as Hvs2'.
-    { apply list_lookup_lookup_total_lt.
-      (* TODO: lia doesn't work here *)
-      rewrite H0. rewrite -(Nat2Z.id n).
-      apply Z2Nat.inj_lt; try lia. }
-
     iModIntro.
-    pose (Ψ1 := (λ v, ⌜v = vs1 !!! Z.to_nat i1⌝ ∗ l1 ↦ₗ∗ vs1)%I).
-    pose (Ψ2 := (λ v, ⌜v = vs2 !!! Z.to_nat i2⌝ ∗ l2 ↦ᵣ∗ vs2)%I).
+    pose (Ψ1 := (λ v, ⌜v = vs1 !!! i1'⌝ ∗ l1 ↦ₗ∗ vs1)%I).
+    pose (Ψ2 := (λ v, ⌜v = vs2 !!! i2'⌝ ∗ l2 ↦ᵣ∗ vs2)%I).
     iApply (dwp_atomic_lift_wp Ψ1 Ψ2 with "[Hl1] [Hl2] [-]").
     { rewrite /TWP1 /Ψ1.
-      assert (i1 < n) by lia.
-      iPoseProof (twp_load_offset _ _ _ (Z.to_nat i1)
-                    (heapG0:=heapG1) with "Hl1") as "HH"; first done.
-      rewrite Z2Nat.id; try lia. (*XXX*)
-      iApply "HH"; eauto. }
+      iApply (twp_load_offset (heapG0:=heapG1) with "Hl1"); eauto. }
     { rewrite /TWP2 /Ψ2.
-      assert (i2 < n) by lia.
-      iPoseProof (twp_load_offset _ _ _ (Z.to_nat i2)
-                    (heapG0:=heapG2) with "Hl2") as "HH"; first done.
-      rewrite Z2Nat.id; try lia. (*XXX*)
-      iApply "HH"; eauto. }
-
-    iIntros (v1 v2). iDestruct 1 as (->) "Hl1". iDestruct 1 as (->) "Hl2".
-    iNext.
-    iAssert (A ξ (vs1 !!! Z.to_nat i1) (vs2 !!! Z.to_nat i1)) as "#HvsA".
-    { iApply (big_sepL2_lookup with "HAs").
-      apply Hvs1. apply Hvs2. }
-    iAssert (A ξ (vs1 !!! Z.to_nat i2) (vs2 !!! Z.to_nat i2)) as "#HvsA'".
-    { iApply (big_sepL2_lookup with "HAs").
-      apply Hvs1'. apply Hvs2'. }
+      iApply (twp_load_offset (heapG0:=heapG2) with "Hl2"); eauto. }
+    iDestruct 1 as (->) "Hl1"; iDestruct 1 as (->) "Hl2". iNext.
+    iAssert (A ξ (vs1 !!! i1') (vs2 !!! i1')) as "#HvsA".
+    { by iApply (big_sepL2_lookup with "HAs"). }
+    iAssert (A ξ (vs1 !!! i2') (vs2 !!! i2')) as "#HvsA'".
+    { by iApply (big_sepL2_lookup with "HAs"). }
     iMod ("Hcl" with "[-]") as "_".
     { iNext. iExists _,_. iFrame "Hl1 Hl2 HAs".
       repeat iSplit; eauto with iFrame. }
     iModIntro. iApply C. iSplit.
-    - rewrite (PR (vs1 !!! Z.to_nat i1)).
+    - rewrite (PR (vs1 !!! i1')).
       iDestruct "HvsA" as "[$ _]".
-    - rewrite (PR (vs1 !!! Z.to_nat i2)).
+    - rewrite (PR (vs1 !!! i2')).
       iDestruct "HvsA'" as "[_ $]".
   Qed.
 
@@ -381,199 +180,50 @@ Section spec.
     iIntros (PR C).
     iDestruct 1 as (l1 l2 n -> ->) "Ha".
     iDestruct 1 as (i1 i2 -> ->) "_".
-    iIntros "#Hdummy".
-    dwp_rec. dwp_pures.
-    repeat case_bool_decide; dwp_pures;
-      try by iApply dwp_value.
-    - iApply array_get_rhs; eauto. lia.
-    - iApply array_get_rhs; eauto. lia.
-    - iApply array_get_rhs; eauto. lia.
-    - iApply array_get_lhs; eauto. lia.
-    - iApply array_get_lhs; eauto. lia.
-    - iApply array_get_lhs; eauto. lia.
-    - iApply array_get_both; eauto; lia.
+    iIntros "#Hd".
+    rewrite /get. dwp_pures.
+    repeat case_bool_decide; dwp_pures; iApply (array_get_both with "Ha"); auto with lia.
   Qed.
 
   (** * Set typing *)
-
-  (** ** Helper lemmas *)
-  Lemma array_set_rhs A ξ v1 v2 l1 l2 i2 n :
+  Lemma lrel_list_update_both A ξ vs1 vs2 (i1 i2 : nat) v1 v2 :
     pseudo_refl A ξ →
     contractible A ξ →
-    0 ≤ i2 < n →
-    A ξ v1 v2 -∗
-    array_inv A ξ l1 l2 n -∗
-    DWP Skip & #(l2 +ₗ i2) <- v2 : ⟦ tunit ⟧ ξ.
-  Proof.
-    iIntros (PR C Hi2) "#Hv Ha".
-    iApply dwp_atomic.
-    iInv (locsN.@(l1, l2)) as
-          (vs1 vs2) "(>% & >% & >Hl1 & >Hl2 & HAs)" "Hcl".
-    rewrite /lrel_list.
-
-    assert (vs1 !! Z.to_nat i2 = Some (vs1 !!! Z.to_nat i2)) as Hvs1.
-    { apply list_lookup_lookup_total_lt.
-      (* TODO: lia doesn't work here *)
-      rewrite H. rewrite -(Nat2Z.id n).
-      apply Z2Nat.inj_lt; try lia. }
-    assert (vs2 !! Z.to_nat i2 = Some (vs2 !!! Z.to_nat i2)) as Hvs2.
-    { apply list_lookup_lookup_total_lt.
-      (* TODO: lia doesn't work here *)
-      rewrite H0. rewrite -(Nat2Z.id n).
-      apply Z2Nat.inj_lt; try lia. }
-
-    iModIntro.
-    pose (vs2' := <[Z.to_nat i2:=v2]>vs2).
-    pose (Ψ1 := (λ v, ⌜v = #()⌝ : iProp Σ)%I).
-    pose (Ψ2 := (λ v, ⌜v = #()⌝ ∗ l2 ↦ᵣ∗ vs2')%I).
-    iApply (dwp_atomic_lift_wp Ψ1 Ψ2 with "[] [Hl2] [-]").
-    { rewrite /TWP1 /Ψ1. wp_pures. done. }
-    { rewrite /TWP2 /Ψ2.
-      assert (i2 < n) by lia.
-      iPoseProof (twp_store_offset _ _ _ (Z.to_nat i2)
-                                   (heapG0:=heapG2) with "Hl2") as "HH".
-      { rewrite Hvs2. eauto. }
-      rewrite Z2Nat.id; try lia. (*XXX*)
-      iApply "HH"; eauto. }
-    iIntros (?? ->). iDestruct 1 as (->) "Hl2".
-    iNext.
-
-    rewrite (big_sepL2_insert_acc _ _ _ (Z.to_nat i2) _) //.
-    iDestruct "HAs" as "[#HvsA HAs]".
-    iSpecialize ("HAs" $! (vs1 !!! Z.to_nat i2) v2 with "[]").
-    { iApply C. iSplit.
-      - rewrite (PR (vs1 !!! _)). iDestruct "HvsA" as "[$ _]".
-      - rewrite (PR v1 v2). iDestruct "Hv" as "[_ $]". }
-
-    iMod ("Hcl" with "[-]") as "_".
-    { iNext. iExists _,_. iFrame "HAs Hl2".
-      rewrite !insert_length.
-      repeat iSplit; eauto.
-      rewrite list_insert_id //. }
-    iModIntro. rewrite interp_eq ; eauto.
-  Qed.
-
-  Lemma array_set_lhs A ξ v1 v2 l1 l2 i1 n :
-    pseudo_refl A ξ →
-    contractible A ξ →
-    0 ≤ i1 < n →
-    A ξ v1 v2 -∗
-    array_inv A ξ l1 l2 n -∗
-    DWP #(l1 +ₗ i1) <- v1 & Skip : ⟦ tunit ⟧ ξ.
-  Proof.
-    iIntros (PR C Hi2) "#Hv Ha".
-    iApply dwp_atomic.
-    iInv (locsN.@(l1, l2)) as
-          (vs1 vs2) "(>% & >% & >Hl1 & >Hl2 & HAs)" "Hcl".
-    rewrite /lrel_list.
-
-    assert (vs1 !! Z.to_nat i1 = Some (vs1 !!! Z.to_nat i1)) as Hvs1.
-    { apply list_lookup_lookup_total_lt.
-      (* TODO: lia doesn't work here *)
-      rewrite H. rewrite -(Nat2Z.id n).
-      apply Z2Nat.inj_lt; try lia. }
-    assert (vs2 !! Z.to_nat i1 = Some (vs2 !!! Z.to_nat i1)) as Hvs2.
-    { apply list_lookup_lookup_total_lt.
-      (* TODO: lia doesn't work here *)
-      rewrite H0. rewrite -(Nat2Z.id n).
-      apply Z2Nat.inj_lt; try lia. }
-
-    iModIntro.
-    pose (vs1' := <[Z.to_nat i1:=v1]>vs1).
-    pose (Ψ1 := (λ v, ⌜v = #()⌝ ∗ l1 ↦ₗ∗ vs1')%I).
-    pose (Ψ2 := (λ v, ⌜v = #()⌝ : iProp Σ)%I).
-    iApply (dwp_atomic_lift_wp Ψ1 Ψ2 with "[Hl1] [] [-]").
-    { rewrite /TWP1 /Ψ1.
-      assert (i1 < n) by lia.
-      iPoseProof (twp_store_offset _ _ _ (Z.to_nat i1)
-                                   (heapG0:=heapG1) with "Hl1") as "HH".
-      { rewrite Hvs1. eauto. }
-      rewrite Z2Nat.id; try lia. (*XXX*)
-      iApply "HH"; eauto. }
-    { rewrite /TWP2 /Ψ2. by wp_pures. }
-    iIntros (??). iDestruct 1 as (->) "Hl1". iIntros (->).
-    iNext.
-
-    rewrite (big_sepL2_insert_acc _ _ _ (Z.to_nat i1) _) //.
-    iDestruct "HAs" as "[#HvsA HAs]".
-    iSpecialize ("HAs" $! v1 (vs2 !!! Z.to_nat i1) with "[]").
-    { iApply C. iSplit.
-      - rewrite (PR v1 v2). iDestruct "Hv" as "[$ _]".
-      - rewrite (PR (vs1 !!! _)). iDestruct "HvsA" as "[_ $]". }
-
-    iMod ("Hcl" with "[-]") as "_".
-    { iNext. iExists _,_. iFrame "HAs Hl1".
-      rewrite !insert_length.
-      repeat iSplit; eauto.
-      rewrite list_insert_id //. }
-    iModIntro. rewrite interp_eq ; eauto.
-  Qed.
-
-  Lemma lrel_list_update_both A ξ vs1 vs2 i1 i2 v1 v2 :
-    pseudo_refl A ξ →
-    contractible A ξ →
-    0 ≤ i1 < List.length vs1 →
-    0 ≤ i2 < List.length vs2 →
+    (i1 < List.length vs1)%nat →
+    (i2 < List.length vs2)%nat →
     A ξ v1 v2 -∗
     ([∗ list] v0;v3 ∈ vs1;vs2, A ξ v0 v3) -∗
-    [∗ list] v0;v3 ∈ <[Z.to_nat i1:=v1]>vs1;<[Z.to_nat i2:=v2]>vs2, A ξ v0 v3.
+    [∗ list] v0;v3 ∈ <[i1:=v1]>vs1;<[i2:=v2]>vs2, A ξ v0 v3.
   Proof.
     iIntros (PR C Hi1 Hi2) "#Hv HAs".
     iDestruct (big_sepL2_length with "HAs") as %Hfoo.
-
-    assert (vs1 !! Z.to_nat i1 = Some (vs1 !!! Z.to_nat i1)) as Hvs1.
-    { apply list_lookup_lookup_total_lt.
-      (* TODO: lia doesn't work here *)
-      rewrite -(Nat2Z.id (List.length vs1)).
-      apply Z2Nat.inj_lt; try lia. }
-    assert (vs1 !! Z.to_nat i2 = Some (vs1 !!! Z.to_nat i2)) as Hvs1'.
-    { apply list_lookup_lookup_total_lt.
-      (* TODO: lia doesn't work here *)
-      rewrite -(Nat2Z.id (List.length vs1)).
-      apply Z2Nat.inj_lt; try lia. }
-    assert (vs2 !! Z.to_nat i1 = Some (vs2 !!! Z.to_nat i1)) as Hvs2.
-    { apply list_lookup_lookup_total_lt.
-      (* TODO: lia doesn't work here *)
-      rewrite -(Nat2Z.id (List.length vs2)).
-      apply Z2Nat.inj_lt; try lia. }
-    assert (vs2 !! Z.to_nat i2 = Some (vs2 !!! Z.to_nat i2)) as Hvs2'.
-    { apply list_lookup_lookup_total_lt.
-      (* TODO: lia doesn't work here *)
-      rewrite -(Nat2Z.id (List.length vs2)).
-      apply Z2Nat.inj_lt; try lia. }
-
     destruct (decide (i1 = i2)) as [<-|Hi1i2].
     - (* If the indices at which we insert are the same,
          then it's fairly straightforward *)
-      rewrite (big_sepL2_insert_acc _ _ _ (Z.to_nat i1) _) //.
+      rewrite (big_sepL2_insert_acc _ _ _ i1) //.
       iDestruct "HAs" as "[#HvsA HAs]".
       iApply ("HAs" $! v1 v2 with "Hv").
     - (* Otherwise we need to do two insertions *)
-      rewrite (big_sepL2_insert_acc _ _ _ (Z.to_nat i1) _) //.
+      rewrite (big_sepL2_insert_acc _ _ _ i1) //.
       iDestruct "HAs" as "[#HvsA HAs]".
-      iSpecialize ("HAs" $! v1 (vs2 !!! Z.to_nat i1) with "[]").
+      iSpecialize ("HAs" $! v1 (vs2 !!! i1) with "[]").
       { iApply C. iSplit.
         - rewrite (PR v1 v2). iDestruct "Hv" as "[$ _]".
         - rewrite (PR (vs1 !!! _)). iDestruct "HvsA" as "[_ $]". }
       rewrite (list_insert_id vs2) //.
       iClear "HvsA".
-      pose (vs1' := <[Z.to_nat i1:=v1]> vs1).
-
-      rewrite (big_sepL2_insert_acc _ _ _ (Z.to_nat i2) _) //; last first.
-      { rewrite list_lookup_insert_ne //. intros ?%Z2Nat.inj; lia. }
+      rewrite (big_sepL2_insert_acc _ _ _ i2) //; last first.
+      { by rewrite list_lookup_insert_ne. }
       iDestruct "HAs" as "[#HvsA HAs]".
-      iSpecialize ("HAs" $! (vs1'!!!Z.to_nat i2) v2 with "[]").
-      { assert (vs1' !!! Z.to_nat i2 = vs1 !!! Z.to_nat i2) as ->.
-        { rewrite list_lookup_total_insert_ne//.
-          intros ?%Z2Nat.inj; lia. }
+      iSpecialize ("HAs" $! (<[i1:=v1]> vs1 !!! i2) v2 with "[]").
+      { assert (<[i1:=v1]> vs1 !!! i2 = vs1 !!! i2) as ->.
+        { by rewrite list_lookup_total_insert_ne. }
         iApply C. iSplit.
         - rewrite (PR (vs1 !!! _)). iDestruct "HvsA" as "[$ _]".
         - rewrite (PR v1 v2). iDestruct "Hv" as "[_ $]". }
-      rewrite (list_insert_id vs1') //.
+      rewrite (list_insert_id (<[i1:=v1]> vs1)) //.
       apply list_lookup_lookup_total_lt.
-      rewrite insert_length. rewrite Hfoo.
-      rewrite -(Nat2Z.id (List.length vs2)).
-      apply Z2Nat.inj_lt; try lia.
+      rewrite insert_length. lia.
   Qed.
 
   Lemma array_set_both A ξ v1 v2 l1 l2 i1 i2 n :
@@ -586,59 +236,30 @@ Section spec.
     DWP #(l1 +ₗ i1) <- v1 & #(l2 +ₗ i2) <- v2 : ⟦ tunit ⟧ ξ.
   Proof.
     iIntros (PR C Hi1 Hi2) "#Hv Ha".
+    assert (∃ i1' : nat, i1 = i1' ∧ i1' < n)%nat as (i1' & -> & ?)
+      by (exists (Z.to_nat i1); lia).
+    assert (∃ i2' : nat, i2 = i2' ∧ i2' < n)%nat as (i2' & -> & ?)
+      by (exists (Z.to_nat i2); lia).
     iApply dwp_atomic.
     iInv (locsN.@(l1, l2)) as
           (vs1 vs2) "(>% & >% & >Hl1 & >Hl2 & HAs)" "Hcl".
-    rewrite /lrel_list.
-
-    assert (vs1 !! Z.to_nat i1 = Some (vs1 !!! Z.to_nat i1)) as Hvs1.
-    { apply list_lookup_lookup_total_lt.
-      (* TODO: lia doesn't work here *)
-      rewrite H. rewrite -(Nat2Z.id n).
-      apply Z2Nat.inj_lt; try lia. }
-    assert (vs2 !! Z.to_nat i2 = Some (vs2 !!! Z.to_nat i2)) as Hvs2.
-    { apply list_lookup_lookup_total_lt.
-      (* TODO: lia doesn't work here *)
-      rewrite H0. rewrite -(Nat2Z.id n).
-      apply Z2Nat.inj_lt; try lia. }
-    assert (vs2 !! Z.to_nat i1 = Some (vs2 !!! Z.to_nat i1)) as Hvs2'.
-    { apply list_lookup_lookup_total_lt.
-      (* TODO: lia doesn't work here *)
-      rewrite H0. rewrite -(Nat2Z.id n).
-      apply Z2Nat.inj_lt; try lia. }
-
     iModIntro.
-    pose (vs1' := <[Z.to_nat i1:=v1]>vs1).
-    pose (vs2' := <[Z.to_nat i2:=v2]>vs2).
-    pose (Ψ1 := (λ v, ⌜v = #()⌝ ∗ l1 ↦ₗ∗ vs1')%I).
-    pose (Ψ2 := (λ v, ⌜v = #()⌝ ∗ l2 ↦ᵣ∗ vs2')%I).
+    pose (Ψ1 v := (⌜v = #()⌝ ∗ l1 ↦ₗ∗ <[i1':=v1]>vs1)%I).
+    pose (Ψ2 v := (⌜v = #()⌝ ∗ l2 ↦ᵣ∗ <[i2':=v2]>vs2)%I).
     iApply (dwp_atomic_lift_wp Ψ1 Ψ2 with "[Hl1] [Hl2] [-]").
     { rewrite /TWP1 /Ψ1.
-      assert (i1 < n) by lia.
-      iPoseProof (twp_store_offset _ _ _ (Z.to_nat i1)
-                                   (heapG0:=heapG1) with "Hl1") as "HH".
-      { rewrite Hvs1. eauto. }
-      rewrite Z2Nat.id; try lia. (*XXX*)
-      iApply "HH"; eauto. }
+     iApply (twp_store_offset (heapG0:=heapG1) with "Hl1"); eauto. }
     { rewrite /TWP2 /Ψ2.
-      assert (i2 < n) by lia.
-      iPoseProof (twp_store_offset _ _ _ (Z.to_nat i2)
-                                   (heapG0:=heapG2) with "Hl2") as "HH".
-      { rewrite Hvs2. eauto. }
-      rewrite Z2Nat.id; try lia. (*XXX*)
-      iApply "HH"; eauto. }
+      iApply (twp_store_offset (heapG0:=heapG2) with "Hl2"); eauto. }
+    iDestruct 1 as (->) "Hl1". iDestruct 1 as (->) "Hl2". iNext.
 
-    iIntros (??). iDestruct 1 as (->) "Hl1". iDestruct 1 as (->) "Hl2".
-    iNext.
-
-    iDestruct (lrel_list_update_both _ _ _ _ i1 i2 with "Hv HAs") as "HAs";
-      (lia || eauto).
+    iDestruct (lrel_list_update_both _ _ _ _ i1' i2' with "Hv HAs") as "HAs";
+      eauto with lia.
 
     iMod ("Hcl" with "[-]") as "_".
     { iNext. iExists _,_. iFrame "HAs Hl1".
-      rewrite !insert_length.
-      repeat iSplit; eauto. }
-    iModIntro. rewrite interp_eq ; eauto.
+      rewrite !insert_length. eauto 10. }
+    iModIntro. rewrite interp_eq; eauto.
   Qed.
 
   (** ** The main 'set' typing *)
@@ -653,17 +274,9 @@ Section spec.
     iIntros (PR C).
     iDestruct 1 as (l1 l2 n -> ->) "Ha".
     iDestruct 1 as (i1 i2 -> ->) "_".
-    iIntros "#Hv".
-    dwp_rec. dwp_pures.
+    iIntros "#Hd".
+    rewrite /set. dwp_pures.
     repeat case_bool_decide; dwp_pures;
-      try iApply logrel_unit.
-    - iApply (array_set_rhs with "Hv Ha"); eauto. lia.
-    - iApply (array_set_rhs with "Hv Ha"); eauto. lia.
-    - iApply (array_set_rhs with "Hv Ha"); eauto. lia.
-    - iApply (array_set_lhs with "Hv Ha"); eauto. lia.
-    - iApply (array_set_lhs with "Hv Ha"); eauto. lia.
-    - iApply (array_set_lhs with "Hv Ha"); eauto. lia.
-    - iApply (array_set_both with "Hv Ha"); eauto; lia.
+      iApply (array_set_both with "Hd Ha"); auto with lia.
   Qed.
-
 End spec.
